rules/proof.v
@@ -1,0 +1,100 @@
+(*
+
+  Copyright 2014 Cornell University
+  Copyright 2015 Cornell University
+
+  This file is part of VPrl (the Verified Nuprl project).
+
+  VPrl is free software: you can redistribute it and/or modify
+  it under the terms of the GNU General Public License as published by
+  the Free Software Foundation, either version 3 of the License, or
+  (at your option) any later version.
+
+  VPrl is distributed in the hope that it will be useful,
+  but WITHOUT ANY WARRANTY; without even the implied warranty of
+  MERCHANTABILITY or FITNESS FOR A PARTICULAR PURPOSE.  See the
+  GNU General Public License for more details.
+
+  You should have received a copy of the GNU General Public License
+  along with VPrl.  If not, see <http://www.gnu.org/licenses/>.
+
+
+  Website: http://nuprl.org/html/verification/
+  Authors: Abhishek Anand & Vincent Rahli & Mark Bickford
+
+*)
+
+
+Require Export rules_isect.
+
+Inductive valid_rule {o} : @rule o -> Type :=
+| valid_rule_isect_equality :
+    forall a1 a2 b1 b2 x1 x2 y i H,
+      !LIn y (vars_hyps H)
+      -> valid_rule (rule_isect_equality a1 a2 b1 b2 x1 x2 y i H).
+
+Inductive gen_proof {o} (G : @baresequent o) : Type :=
+| gen_proof_cons :
+    forall hyps args,
+      valid_rule (mk_rule G hyps args)
+      -> (forall h, LIn h hyps -> gen_proof h)
+      -> gen_proof G.
+
+(* [pwf_sequent] says that the hypotheses and conclusion are well-formed and
+   the type is closed w.r.t. the hypotheses.
+ *)
+Lemma valid_gen_proof {o} :
+  forall lib (seq : @baresequent o) (wf : pwf_sequent seq),
+    gen_proof seq -> sequent_true2 lib seq.
+Proof.
+  introv wf p.
+  induction p as [? ? ? vr imp ih].
+  inversion vr as [a1 a2 b1 b2 x1 x2 y i hs niy]; subst; allsimpl; clear vr.
+
+  - apply (rule_isect_equality_true2 lib y i a1 a2 b1 b2 x1 x2 hs); simpl; tcsp.
+
+    + unfold args_constraints; simpl; introv h; repndors; subst; tcsp.
+
+    + introv e; repndors; subst; tcsp.
+
+      * apply ih; auto.
+        apply (rule_isect_equality_wf y i a1 a2 b1 b2 x1 x2 hs); simpl; tcsp.
+
+      * apply ih; auto.
+        apply (rule_isect_equality_wf y i a1 a2 b1 b2 x1 x2 hs); simpl; tcsp.
+Qed.
+
+Inductive proof {o} : @baresequent o -> Type :=
+| proof_cons :
+    forall a1 a2 b1 b2 x1 x2 y i H,
+      !LIn y (vars_hyps H)
+      -> proof (rule_isect_equality_hyp1 a1 a2 i H)
+      -> proof (rule_isect_equality_hyp2 a1 b1 b2 x1 x2 y i H)
+      -> proof (rule_isect_equality_concl a1 a2 x1 x2 b1 b2 i H).
+
+Lemma valid_proof {o} :
+  forall lib (seq : @baresequent o) (wf : pwf_sequent seq),
+    proof seq -> sequent_true2 lib seq.
+Proof.
+  introv wf p.
+  induction p as [a1 a2 b1 b2 x1 x2 y i hs niy p1 ih1 p2 ih2]; allsimpl.
+
+  - apply (rule_isect_equality_true2 lib y i a1 a2 b1 b2 x1 x2 hs); simpl; tcsp.
+
+    + unfold args_constraints; simpl; introv h; repndors; subst; tcsp.
+
+    + introv e; repndors; subst; tcsp.
+
+      * apply ih1; auto.
+        apply (rule_isect_equality_wf y i a1 a2 b1 b2 x1 x2 hs); simpl; tcsp.
+
+      * apply ih2; auto.
+        apply (rule_isect_equality_wf y i a1 a2 b1 b2 x1 x2 hs); simpl; tcsp.
+Qed.
+
+
+(*
+*** Local Variables:
+*** coq-load-path: ("." "../util/" "../terms/" "../computation/" "../cequiv/" "../close/" "../per/")
+*** End:
+*)
